CaseStudy/ifc_SO/Testing/GenerationProofs.v
@@ -1,6 +1,6 @@
 Require Import QuickChick SetOfOutcomes.
 
-Require Import Common Machine Generation.
+Require Import Common Machine Generation. 
 
 Require Import List.
 Require Import ZArith.
@@ -9,10 +9,9 @@ Require Import ssreflect ssrbool ssrnat eqtype.
 
 
 Lemma gen_from_length_correct: forall l,
-  peq (gen_from_length l) (fun z => (Z.le 0 z /\ Z.le z (l-1))).
+  (gen_from_length l) <--> (fun z => (Z.le 0 z /\ Z.le z (l-1))).
 Proof.
-  move => l. Opaque Z.compare. 
-  rewrite /peq /gen_from_length /choose /PredMonad /cmp /=. 
+  move => l z. rewrite /gen_from_length choose_def. 
   split => [[/Z.compare_le_iff H1 /Z.compare_ge_iff H2]|
             [/Z.compare_le_iff H1 /Z.compare_ge_iff H2]];
     by split; auto.
@@ -20,19 +19,20 @@ Qed.
 
 
 Lemma gen_from_nat_length_correct: forall l,
-  peq (gen_from_nat_length l) (fun z => (Z.le 0 z /\ Z.le z ((Z.of_nat l)-1))).
+  (gen_from_nat_length l) <--> (fun z => (Z.le 0 z /\ Z.le z ((Z.of_nat l)-1))).
 Proof.
-  move => l.
-  rewrite /gen_from_nat_length.
+  move => l z.
+  rewrite /gen_from_nat_length. 
   move/(_ (Z.of_nat l)): gen_from_length_correct; apply. 
 Qed.
 
 Lemma gen_BinOpT_correct : 
   peq gen_BinOpT all.
 Proof.
-  rewrite /peq /gen_BinOpT /all. split => // _.
-  apply oneof_correct. left. 
-  case : A; [exists (pure BAdd) | exists (pure BMult)]; split => //=;
+  rewrite /gen_BinOpT /all. move => op. 
+  split => // _.  
+  apply oneof_equiv. left. 
+  case : op; [exists (pure BAdd) | exists (pure BMult)]; split => //=;
   [|right]; by left.
 Qed.
 
@@ -46,13 +46,13 @@ Qed.
 
 Lemma gen_label_correct : 
   forall (l : Label),
-    peq (gen_label l) (fun e => In e (allThingsBelow l)).
+    (gen_label l) <--> (fun e => In e (allThingsBelow l)).
 Proof.
-  move=> l. rewrite /peq /gen_label. move => l'.   
-  split => [/elements_correct [H1 | [H1 H2]] //= | HIn]; subst.  
+  move=> l. rewrite /gen_label. move => l'. 
+  split => [/elements_equiv [H1 | [H1 H2]] //= | HIn]; subst.   
   + rewrite /allThingsBelow  /allBelow in H1. apply map_eq_nil in H1.
     by move/powerset_nonempty : H1.
-  + apply elements_correct. by left.
+  + apply elements_equiv. by left.
 Qed.
 
 Lemma gen_label_inf_correct : forall inf,
@@ -60,3 +60,423 @@ Lemma gen_label_inf_correct : forall inf,
 Proof.
   move => inf. apply/gen_label_correct.
 Qed.
+
+Lemma gen_PC_correct: 
+  forall inf, 
+    (gen_PC inf) <--> (fun pc => let '(PAtm z l) := pc in
+                                 (In l (allThingsBelow (top_prin inf))) /\ 
+                                 (0 <= z <= (code_len inf) - 1)%Z).
+Proof.
+  move=> inf ptr. rewrite /gen_PC.
+  split.
+  + rewrite bindGen_def. move => [lab [/gen_label_inf_correct gen_lab H]].
+    rewrite bindGen_def in H. move : H => [z [/gen_from_length_correct H1 Hret]].
+    rewrite returnGen_def in Hret. subst. by split.
+  + case : ptr => z l. move => [Hin Hrng]. 
+    rewrite bindGen_def. exists l; split.
+    by apply /gen_label_inf_correct.
+    rewrite bindGen_def. exists z; split => //.
+    by apply /gen_from_length_correct.
+Qed.
+
+
+Definition val_spec (inf : Info) (v : Value) :=
+  match v with 
+    | Vint _ => True
+    | Vptr ptr =>
+      let '(Ptr mf addr) := ptr in
+      (exists len, In (mf, len) (data_len inf) /\ 
+                   (0 <= addr <= len - 1)%Z) 
+    | Vcptr z => (0 <= z <= (code_len inf) - 1)%Z
+    | Vlab l => In l (allThingsBelow (top_prin inf))
+  end.
+
+(* Move it at arbitrary.v ? *)
+Lemma arbInt_correct : 
+  arbitrary <--> (fun (z : Z) => True).
+Proof.
+  rewrite /arbitrary /arbInt /arbitraryZ.  
+  rewrite sized_def. move => z. split => //= _. 
+  exists (Z.abs_nat z).
+  split. 
+  + apply/Z.compare_le_iff. rewrite Nat2Z.inj_abs_nat. 
+    by case: z => //= p; omega. 
+  + apply/Z.compare_ge_iff. rewrite Nat2Z.inj_abs_nat. 
+    by case: z => //= p; omega. 
+Qed.
+
+(* I don't know if this is reasonable, but otherwise some generators are 
+  broken (suck as gen_Pointer) *)
+
+Axiom data_len_nonempty : forall (inf : Info), data_len inf <> [].
+
+Lemma gen_Pointer_correct: 
+  forall inf, 
+    (gen_Pointer inf) <--> (fun ptr => 
+                              let '(Ptr mf addr) := ptr in
+                              (exists len, In (mf, len) (data_len inf) /\ 
+                                           (0 <= addr <= len - 1)%Z)). 
+Proof.
+  move => inf ptr. 
+  move: (data_len_nonempty inf) => non_empty. 
+  case: inf non_empty => def clen dlen top regs non_empty. rewrite /gen_Pointer.
+  split.
+  * rewrite bindGen_def. move => [[mf z] [/elements_equiv Helem  H]].
+    rewrite bindGen_def in H. move : H => [a [/gen_from_length_correct H Hret]].
+    rewrite returnGen_def in Hret; subst.
+    simpl. case : Helem => [HIn | [Heq1 [Heq2 Heq3]]]; subst.
+    by exists z. omega.
+  * case: ptr => mf z. 
+    case: dlen {non_empty} =>  [| x xs].
+    - rewrite bindGen_def. 
+      move=> [len  [//= HIn Hrng]].
+    -  Opaque bindGen choose Z.compare returnGen. 
+       move=> [len  [//= HIn [Hrng1 Hrng2]]].
+       rewrite bindGen_def.  
+       exists (mf, len). split.
+       apply/elements_equiv. by left. 
+       rewrite bindGen_def. 
+       exists z. split => //. split. by apply/Z.compare_le_iff.
+       by apply/Z.compare_ge_iff.
+Qed.
+
+Lemma gen_value_correct: 
+  forall inf,
+    (gen_Value inf) <--> (val_spec inf).
+Proof.
+  rewrite /gen_Value /val_spec.
+  case=> def clen dlen top regs. case.
+  + (* VInt *)
+    move => z. split => // _. apply/frequency_equiv.
+    left. exists 1. eexists. split. by constructor.
+    split => //.
+    rewrite liftGen_def. eexists; split => //.
+    apply/frequency_equiv. left.
+    exists 10. exists arbitrary. split. by constructor.
+    split => //. by apply/arbInt_correct.
+  + (* Vptr *)  
+    case => mf addr. 
+    split. Opaque bindGen choose Z.compare returnGen gen_Pointer.    
+    - move/frequency_equiv => [[n [ g [H1 [H2 H3]]]] | [[// | H1] H2]]. 
+      * case:H1 => [[Heq1 Heq2] | [[Heq1 Heq2] | [[Heq1 Heq2] | [[Heq1 Heq2] | //]]]];
+        subst; try (rewrite liftGen_def in H2; move : H2 => [a [H2 H2']]); 
+        try discriminate.      
+        move/gen_Pointer_correct: H2 H2' => H2 [H2']; subst.
+        move : H2 => //= [len [ HIn Hrng]].  
+      * by rewrite liftGen_def in H2; move : H2 => [a [H2 H2']].
+    - move => [len [HIn [Hrng1 Hrg2]]].
+      apply/frequency_equiv. left. exists 1. eexists. 
+      split. apply in_cons.  apply in_cons. constructor. 
+      reflexivity.
+      rewrite liftGen_def. split => //. eexists.
+      split => //. apply gen_Pointer_correct. by exists len.
+   + (* Vcptr *)
+     move => addr. split. 
+     - move/frequency_equiv => [[n [g [H1 [H2 H3]]]] | [H1 H2]]. 
+       * case: H1 => [[Heq1 Heq2] | [[Heq1 Heq2] | [[Heq1 Heq2] | [[Heq1 Heq2] | //]]]];
+         subst; try (rewrite liftGen_def in H2; move : H2 => [a [H2 H2']]); 
+         try discriminate.
+         move : H2 H2' => [/Z.compare_le_iff H1 /Z.compare_ge_iff H2] [H2']; subst.
+         by split.
+       * by rewrite liftGen_def in H2; move : H2 => [a [H2 H2']].
+     - move => [/=  H1  H2].
+       apply/frequency_equiv. left. exists 1. eexists. split. 
+       apply in_cons. constructor. 
+       reflexivity. 
+       rewrite liftGen_def. split => //. exists addr. split => //=. 
+       split. by apply/Z.compare_le_iff.
+       by apply/Z.compare_ge_iff.
+   + (* Vlab *)
+     move => L. split.
+     - move/frequency_equiv => [[n [g [H1 [H2 H3]]]] | [H1 H2]].
+       * case: H1 => [[Heq1 Heq2] | [[Heq1 Heq2] | [[Heq1 Heq2] | [[Heq1 Heq2] | //]]]];
+         subst; try (rewrite liftGen_def in H2; move : H2 => [a [H2 H2']]); 
+         try discriminate.
+         by move : H2 H2' => /gen_label_inf_correct H1 [H2']; subst.
+       * by rewrite liftGen_def in H2; move : H2 => [a [H2 H2']].
+     - move => H. apply/frequency_equiv. left. exists 1. eexists.
+       split. apply in_cons. apply in_cons. apply in_cons. constructor. 
+       reflexivity.
+       rewrite liftGen_def. split => //. exists L. split => //=.
+       by apply/gen_label_inf_correct.
+Qed.
+      
+        
+Lemma gen_atom_correct:
+  forall inf,
+    (gen_atom inf) <--> (fun atm =>
+                           let '(Atm val lab) := atm in
+                           val_spec inf val /\ 
+                           In lab (allThingsBelow (top_prin inf))).
+Proof.
+  move => inf atm. rewrite /gen_atom /liftGen2 bindGen_def. case: atm => val lab. 
+  split. 
+  + move => [val' [/gen_value_correct Hval Hbind]].
+    rewrite bindGen_def in Hbind.
+    move : Hbind => [lab' [/gen_label_inf_correct Hlab Hret]].
+    rewrite returnGen_def in Hret. 
+    by move : Hret => [Heq1 Heq2]; subst.
+  + move => [Hval Hlab].
+    exists val. split; [by apply/gen_value_correct| ].
+    rewrite bindGen_def. exists lab. split => //.
+    by apply/gen_label_inf_correct.
+Qed.
+  
+Definition regs_spec inf regs :=
+  (length regs = no_regs inf) /\
+  (forall reg, 
+     In reg regs ->
+     let '(Atm val lab) := reg in
+     val_spec inf val /\ 
+     In lab (allThingsBelow (top_prin inf))).
+Lemma gen_registers_correct:
+  forall inf,
+    (gen_registers inf) <--> (regs_spec inf).
+Proof.    
+  move => inf regs. 
+  rewrite /gen_registers. split.
+  + move /vectorOf_equiv => [H1 H2].
+    split => //. move => reg HIn. by apply/gen_atom_correct; apply H2. 
+  + move => [Hlen Hregs]. apply/vectorOf_equiv. split => // x HIn.
+    apply/gen_atom_correct. by apply Hregs.
+Qed.
+
+
+Lemma smart_gen_stack_loc_correct :
+  forall f g l1 l2 inf, 
+    (f l1 l2) <--> (g l1 l2) ->
+    (smart_gen_stack_loc f l1 l2 inf) <--> 
+    (fun t =>
+       let '(ptr_a, lab, regs, ptr_r) := t in
+       In lab (allThingsBelow (top_prin inf)) /\
+       regs_spec inf regs /\
+       (0 <= ptr_r <= (Z.of_nat (no_regs inf) - 1))%Z /\
+       let 'PAtm addr lab' := ptr_a in
+       (0 <= addr <= ((code_len inf) - 1))%Z /\
+       g l1 l2 lab').
+Proof.
+  move=> f g l1 l2.
+  case=> def clen dlen top noregs Hequiv. 
+  rewrite /smart_gen_stack_loc /smart_gen /bindGen /returnGen /PredMonad /bindP /returnP //=.
+  move => [[[ptr_a lab] regs] ptr_r]. split.
+  + move =>  
+    [regs' [/gen_registers_correct Hregs [ptr_a' [[lab' [/gen_label_inf_correct Hlab H']]
+                                                  [z [[/Z.compare_le_iff H1 /Z.compare_ge_iff H2] H]]]]]].
+    move: H => [a [/gen_label_inf_correct Hlab' [lab'' [fl1l2 Hret]]]].
+    case: ptr_a' lab' Hret Hlab H' => addr_a' lab_a' lab' Hret' Hlab H'.
+    move : Hret' => [Heq1 Heq2 Heq3 Heq4]; subst.
+    rewrite  /bindGen /returnGen /PredMonad /bindP /returnP //= in H'.
+    move: H' => [z' [[/Z.compare_le_iff H1' /Z.compare_ge_iff H2'] [Heq1 Heq2]]]; subst.
+    repeat (split  => //=; by auto). split => //=. split => //=. split => //=.
+    split => //=. auto. auto. by apply Hequiv.
+  + case: ptr_a. move => addr_a l_a [H1 [H2 [[H3 H3'] [[H4 H5] H6]]]].
+    eexists; split. by apply/gen_registers_correct. 
+    eexists; split. exists lab. split.
+    by apply /gen_label_inf_correct.
+    rewrite bindGen_def. 
+    exists addr_a. split. 
+    split. by apply/Z.compare_le_iff. 
+    by apply/Z.compare_ge_iff. rewrite returnGen_def. reflexivity.
+    exists ptr_r. split. split. 
+    by apply/Z.compare_le_iff. by apply/Z.compare_ge_iff.
+    exists lab. split. by apply /gen_label_inf_correct.
+    exists l_a. split => //=. by apply Hequiv.
+Qed.
+
+
+Lemma allThingsBelow_isLow : 
+  forall l l', 
+    In l (allThingsBelow l') -> l <: l'.
+Proof.
+  move=> l l' /in_map_iff H. rewrite /allThingsBelow /allBelow  in H.  
+  apply Zset.incl_spec.  
+  move=> a HIn. subst.  
+  remember (Zset.elements l) as lst.
+  remember (Zset.elements l') as lst'. 
+  move : H => [x [Heq HIn']]. 
+  
+  
+Lemma elements__label_of_list: 
+  forall lst, Zset.elements (fold_left (fun a b => Zset.add b a) lst Zset.empty) = lst.
+Proof.
+  elim => [| x xs IHxs]. 
+  + by rewrite /label_of_list /= Zset.elements_empty. 
+  + rewrite /label_of_list //= in IHxs *. Search _ (Zset.elements _). a`rewrite IHxs.
+Lemma elements_of_list:
+  forall (l : Label) lst, In l (map label_of_list lst) <-> In (Zset.elements l) lst.
+Proof.
+  move => l lst. split.
+  move/in_map_iff => [zs [Heq HIn]]. 
+  have: 
+H. 
+apply in_map in H.
+  
+  have H: In l 
+
+  remember (l <: l'). case: b Heqb => // Heqb.
+  symmetry in Heqb. apply In_split in H.
+  move : H => [l1 [l2 Heq]]. 
+  rewrite /flows /ZsetLat in Heqb. Search _ (map _ _). 
+  
+  rewrite /label_of_list in H.
+  
+  move : (Heqb) => joinl. move : (Heqb) => joinr.
+  
+  eapply not_flows_not_join_flows_left in joinl.
+  eapply not_flows_not_join_flows_right in joinr.
+  rewrite /flows /join /ZsetLat in joinl joinr.
+  Search _ (incl _ _).
+  apply in_map_iff in H.
+  
+  apply Zset.incl_spec.  
+  remember (Zset.elements l') as lst. 
+  case: lst  l l' Heqlst H => //= [| x xs]  l l' Heqlst H .
+  + case: H => [H | H] //=; subst. by rewrite Zset.elements_empty.
+  + rewrite map_app /= in H. 
+    apply in_app_or in H. 
+    remember (Zset.elements l) as lst'.
+    elim : lst' Heqlst' => //= [|y ys IHys] Heqlst'. 
+    by apply/incl_tl.
+    
+    
+    Search _ (incl _ _).
+
+    move: H => [/in_map_iff H | /in_map_iff H]. 
+    
+      in H. Search _ map.
+    Search _ (In _ _). _ (map _ _) (cons _).
+    Search _ (incl _ _). 
+    apply incl_tl. eapply IHxs.
+  move : H => /in_map_iff H.
+  Search _ (In _ (map _ _)).
+  remember (powerset (Zset.elements l')) as lst.
+  case: lst Heqlst H => [| x xs] Heqlst H.
+  by move: (powerset_nonempty (Zset.elements l')); contradiction.
+  simpl in H. move : H => [H | H].
+  elim : x Heqlst H => //= [|z zs] Heqlst H. 
+  simpl in H. Search _ Zset.empty.
+  
+  apply IHxs.
+  Search _ (In (map _).
+
+Lemma gen_label_between_lax_correct :
+  forall l1 l2,
+    (gen_label_between_lax l1 l2) <--> (fun l => l1 <: l /\ l <: l2).
+Proof.
+  move=> l1 l2 l. rewrite /gen_label_between_lax. split.
+  + move /elements_equiv => [/filter_In [HIn Ht] | [Hempty Heq]]; subst.
+   rewrite /allThingsBelow /allBelow in HIn.
+   rewrite /isLow in Ht. rewrite Ht. 
+   compute in HIn. Search _ (label_of_list _).
+    Search _ allThingsBelow.
+       
+(* Main theorem *)
+Require Import Indist.
+
+Axiom trace_axiom: forall {A} x (y : A), Property.trace x y = y.
+Lemma MemEqDec : forall fp, Mem.EqDec_block fp fp.
+Proof. admit. Qed.
+
+
+Lemma combine_l : forall {A} (l : list A) x y, 
+                    In (x, y) (combine l l) -> x = y.
+Proof. admit. Qed.
+
+Lemma incl_empty : forall s, Zset.incl Zset.empty s.
+Proof.
+  move=> s. apply Zset.incl_spec. by rewrite Zset.elements_empty. 
+Qed.
+
+Lemma incl_same : forall s, Zset.incl s s.
+Proof.
+  move => s.
+  by apply/Zset.incl_spec/incl_refl. 
+Qed.
+
+Require Import ZArith.
+
+Lemma forallb_indist : 
+  forall (l : list frame),
+    forallb
+      (fun x : frame * frame =>
+         let (f1, f2) := x in indist Zset.empty f1 f2)
+      (combine l l).
+Proof.
+  move => l. apply forallb_forall. case => x y H.
+  apply combine_l in H. subst. case: y => s lab l0. 
+  rewrite /indist /indistFrame /isLow.
+  case: (s <: Zset.empty) =>  //=.  
+  rewrite /label_eq flows_refl /=.
+  case: (Zset.incl lab Zset.empty) =>  //=. 
+  elim : l0 => // x l0 IHl0. simpl.
+  apply/andP. split => //=.
+  case: x => valx labx. rewrite incl_same //=. 
+  rewrite /isHigh /isLow .  
+  case: (labx <: Zset.empty)=> //= .
+  case: valx => //=. 
+  try (by rewrite /Z_eq; move => n ; case (Z.eq_dec n n)).
+  case. move => fp i. apply/andP. split => //. 
+  rewrite /mframe_eq. 
+  admit. (*Arrrrg *)
+  by rewrite /Z_eq; case: (Z.eq_dec i i).
+  (by rewrite /Z_eq; move => n ; case (Z.eq_dec n n)).
+  move => L; apply/andP; split; apply incl_same.
+Qed.
+
+Lemma gen_variation_state_correct :
+  gen_variation_state <--> (fun b =>
+                              let '(Var L s1 s2) := b in
+                              indist L s1 s2 = true).
+Proof. 
+  case => Lab s1 s2. split. rewrite /gen_variation_state. 
+  rewrite bindGen_def. 
+  move => [l1 [Htop H]]. 
+  rewrite bindGen_def in H. 
+  move: H => [[mem mframes] [Hinit H]]. 
+  case: mframes Hinit H => [ | mframe1 mframes] Hinit H.
+  - rewrite returnGen_def /= in H. 
+    move : H => [Heq1 Heq2 Heq3]. subst. 
+    rewrite /indist /indistState /failed_state !trace_axiom //=.
+    rewrite /label_eq /isHigh /isLow /flows. simpl. 
+    have Ht: Zset.incl Zset.empty Zset.empty = true by
+        apply/Zset.incl_spec; rewrite Zset.elements_empty. 
+    rewrite Ht -beq_nat_refl /indistMemHelper. 
+    simpl. by rewrite forallb_indist.
+  - case : mframe1 Hinit H => mf1 Z1 Hinit H1.
+    rewrite bindGen_def in H1.
+    move:  H1 => [ptr_a [sgen H1]]. 
+    rewrite bindGen_def in H1.
+    move:  H1 => [regset [sgen2 H1]]. 
+    rewrite bindGen_def in H1.
+    move:  H1 => [st [sgen3 H1]]. 
+    rewrite bindGen_def in H1.
+    move:  H1 => [memg [sgen4 H1]]. 
+    rewrite bindGen_def in H1.
+    move:  H1 => [instr [sgen5 H1]]. 
+    rewrite bindGen_def in H1.
+    move:  H1 => [lab [sgen6 H1]]. 
+    rewrite bindGen_def in H1.
+    move:  H1 => [ST' [sgen7 H1]].     
+    rewrite returnGen_def in H1.
+    move : H1 => [Heq1 Heq2 Heq3]; subst.
+    rewrite /smart_gen in sgen, sgen2, sgen3, sgen4, sgen5, sgen6, sgen7 .
+    
+    simpl in sgen3.
+ 
+rewrite /label
+  
+  
+Print "_ <: _".
+  Search _ (Property.trace _ _). compute .
+
+  rewrite /gen_init_mem bindGen_def in Hinit.
+  
+  
+  
+
+
+  exists Lab. exists Lab. simpl .
+
+  Search _  (Variation).
+Lemma gen_ptr_correct : forall inf,
+  peq (gen_Pointer inf) (fun ptr => 
