src/AbstractGen.v
@@ -51,76 +51,76 @@ Section Utilities.
           {H : GenMonad Gen}. 
   
   Definition liftGen {A B} (f: A -> B) (a : Gen A) 
-  : Gen B :=
-    bindGen a (fun x =>
-    returnGen (f x)).
+  : Gen B := nosimpl 
+               (bindGen a (fun x =>
+                returnGen (f x))).
 
   Definition liftGen2 {A1 A2 B}
              (C : A1 -> A2 -> B) (m1 : Gen A1) (m2  : Gen A2)
   : Gen B:=
-    bindGen m1 (fun x1 => bindGen m2 (fun x2 => returnGen (C x1 x2))).
+    nosimpl (bindGen m1 (fun x1 => bindGen m2 (fun x2 => returnGen (C x1 x2)))).
 
   Definition liftGen3 {A1 A2 A3 R} (F : A1 -> A2 -> A3 -> R)
            (m1 : Gen A1) (m2 : Gen A2) (m3 : Gen A3) 
 
-  : Gen R :=
+  : Gen R := nosimpl(
     bindGen m1 (fun x1 =>
     bindGen m2 (fun x2 =>
     bindGen m3 (fun x3 =>
-    returnGen (F x1 x2 x3)))).
+    returnGen (F x1 x2 x3))))).
 
   Definition liftGen4 {A1 A2 A3 A4 R}
              (F : A1 -> A2 -> A3 -> A4 -> R)
              (m1 : Gen A1) (m2 : Gen A2) (m3 : Gen A3) (m4: Gen A4)
-  : Gen R :=
+  : Gen R := nosimpl(
     bindGen m1 (fun x1 =>
     bindGen m2 (fun x2 =>
     bindGen m3 (fun x3 =>
     bindGen m4 (fun x4 =>
-    returnGen (F x1 x2 x3 x4))))).
+    returnGen (F x1 x2 x3 x4)))))).
 
   Definition liftGen5 {A1 A2 A3 A4 A5 R} 
              (F : A1 -> A2 -> A3 -> A4 -> A5 -> R)
              (m1 : Gen A1) (m2 : Gen A2) (m3 : Gen A3) (m4: Gen A4) (m5 : Gen A5)
-  : Gen R :=
+  : Gen R := nosimpl(
     bindGen m1 (fun x1 =>
     bindGen m2 (fun x2 =>
     bindGen m3 (fun x3 =>
     bindGen m4 (fun x4 =>
     bindGen m5 (fun x5 =>
-    returnGen (F x1 x2 x3 x4 x5)))))).
+    returnGen (F x1 x2 x3 x4 x5))))))).
 
-  Definition sequenceGen {A : Type} (ms : list (Gen A)) : Gen (list A) :=
+  Definition sequenceGen {A : Type} (ms : list (Gen A)) : Gen (list A) := nosimpl(
     fold_right (fun m m' => bindGen m  (fun x => 
                             bindGen m' (fun xs =>
-                            returnGen (x :: xs)))) (returnGen []) ms.
+                            returnGen (x :: xs)))) (returnGen []) ms).
 
   Fixpoint foldGen {A B : Type} (f : A -> B -> Gen A) (l : list B) (a : A) 
-  : Gen A :=
+  : Gen A := nosimpl(
     match l with
       | [] => returnGen a
       | (x :: xs) => bindGen (f a x) (foldGen f xs)
-    end.
+    end).
 
-  Definition oneof {A : Type} (def: Gen A) (gs : list (Gen A)) : Gen A :=
+  Definition oneof {A : Type} (def: Gen A) (gs : list (Gen A)) : Gen A := nosimpl(
     bindGen (choose (0, length gs - 1))
-            (fun n => nth def gs n).
+            (fun n => nth def gs n)).
 
-  Fixpoint replicate {A : Type} (n : nat) (x : A) : list A :=
+  Fixpoint replicate {A : Type} (n : nat) (x : A) : list A := nosimpl(
     match n with
       | O    => nil
       | S n' => cons x (replicate n' x)
-    end.
+    end).
 
-  Fixpoint freqRep {A : Type} (gs : list (nat * Gen A)) : list (Gen A) :=
+  Fixpoint freqRep {A : Type} (gs : list (nat * Gen A)) : list (Gen A) := nosimpl(
     match gs with
       | nil => nil
       | cons (n, g) t =>
         (nseq n g) ++ freqRep t
-    end.
+    end).
 
-  Definition frequency {A : Type} (def : Gen A) (gs : list (nat * Gen A)) :=
-    oneof def (freqRep gs).
+  Definition frequency {A : Type} (def : Gen A) (gs : list (nat * Gen A)) := nosimpl(
+    oneof def (freqRep gs)).
  
   (* This is the implementation of frequency a la QuickCheck and seems more 
      memory and time efficient. Is there a reason the should stick to the 
@@ -129,32 +129,32 @@ Section Utilities.
      is an undefined behavior. *)
  
     Fixpoint pick {A : Type} (def : Gen A) (n : nat) (xs : list (nat * Gen A)) 
-    : nat * Gen A := 
+    : nat * Gen A := nosimpl(
       match xs with 
         | nil => (0, def)
         | (k, x) :: xs =>  
           if (n < k) then (k, x) 
           else pick def (n - k) xs
-      end.
+      end).
 
   Definition frequency'  {A : Type} (def : Gen A) (gs : list (nat * Gen A)) 
-  : Gen A :=
+  : Gen A := nosimpl(
     let tot := (sumn (map (@fst _ _) gs)) in
     bindGen (choose (0, tot-1)) (fun n =>
-    @snd _ _ (pick def n gs)).
+    @snd _ _ (pick def n gs))).
 
-  Definition vectorOf {A : Type} (k : nat) (g : Gen A) : Gen (list A) :=  
+  Definition vectorOf {A : Type} (k : nat) (g : Gen A) : Gen (list A) := nosimpl(
     fold_right (fun m m' =>
                   bindGen m (fun x => 
                   bindGen m' (fun xs => returnGen (cons x xs)))
-               ) (returnGen nil) (nseq k g).
+               ) (returnGen nil) (nseq k g)).
 
-  Definition listOf {A : Type} (g : Gen A) : Gen (list A) :=
-    sized (fun n => bindGen (choose (0, n)) (fun k => vectorOf k g)).
+  Definition listOf {A : Type} (g : Gen A) : Gen (list A) := nosimpl
+    (sized (fun n => bindGen (choose (0, n)) (fun k => vectorOf k g))).
 
-  Definition elements {A : Type} (def : A) (l : list A) :=
+  Definition elements {A : Type} (def : A) (l : list A) := nosimpl(
     let n := length l in
     bindGen (choose (0, n - 1)) (fun n' => 
-    returnGen (List.nth n' l def)).
+    returnGen (List.nth n' l def))).
 
 End Utilities.
